Coherence/Allocation.v
@@ -466,7 +466,7 @@ Proof.
         eapply disj_1_incl. eapply H14.
         eapply bounded_get in H37. eapply H37. eauto.
         dcr; simpl in *.
-        eapply get_app_le in H36; eauto.
+        eapply get_app_lt_1 in H36; eauto.
         inv_get.
         simpl in H37. rewrite H37. eauto.
         eauto with len.
@@ -659,7 +659,6 @@ Proof.
     pe_rewrite; eauto.
     eapply IHrenamedApart2; eauto using inverse_on_incl.
     pe_rewrite; eauto.
-
   - econstructor; eauto. eapply alpha_exp_rename_injective.
     eapply inverse_on_incl. eapply Exp.freeVars_live; eauto. eauto.
 
@@ -711,7 +710,7 @@ Proof.
           rewrite disjoint_app; split; eauto using bounded_disjoint.
           eapply funConstr_disjoint_globals; eauto.
         }
-        simpl in *. eapply get_app_le in H36.
+        simpl in *. eapply get_app_lt_1 in H36.
         inv_get.
         rewrite H37; eauto. eauto with len.
       * {
