Equiv/CtxEq.v
@@ -4,6 +4,37 @@ Require Export Util Var Val Exp Env Map CSet AutoIndTac IL AllInRel Bisim.
 Set Implicit Arguments.
 Unset Printing Records.
 
+Lemma bisim'r_refl s
+  : forall L E r,
+    bisim'r r (L, E, s) (L, E, s).
+Proof.
+  revert s. pcofix CIH.
+  intros; destruct s; simpl in *; intros.
+  - case_eq (exp_eval E e); intros.
+    + pone_step. right. eapply (CIH); eauto.
+    + pno_step.
+  - case_eq (exp_eval E e); intros.
+    case_eq (val2bool v); intros.
+    + pone_step. right. eapply (CIH s1); eauto.
+    + pone_step. right. eapply (CIH s2); eauto.
+    + pno_step.
+  - edestruct (get_dec L (counted l)) as [[b]|].
+    decide (length Y = length (I.block_Z b)).
+    case_eq (omap (exp_eval E) Y); intros.
+    + pone_step. right. eapply CIH.
+    + pno_step.
+    + pno_step.
+    + pno_step; eauto.
+  - pno_step.
+  - case_eq (omap (exp_eval E) Y); intros.
+    + pextern_step.
+      * right. eapply (CIH s); eauto.
+      * right. eapply (CIH s); eauto.
+    + pno_step.
+  - pone_step. right.
+    eapply (CIH s0); eauto using sawtooth_F_mkBlocks.
+Qed.
+
 Instance SR : ProofRelation (params) := {
    ParamRel G Z Z' := Z = Z' /\ Z = G;
    ArgRel V V' G VL VL' := V = V' /\ VL = VL' /\ length VL = length G;
